{\def\g{\gamma_g}
\noindent {\it Proof.} Consider $g(t)=f(x(t)) - \hat f(x(t))$ along the line
segment $x(t)=(1-t)x_0 + tx_j$, $0\le t\le1$, from $x_0$ to $x_j$.  Observe
that $g(0)=f(x_0) - \hat f(x_0) = 0$, $g(1)=f(x_j) - \hat f(x_j) = 0$,
and $g'(t)$ is $\g$-Lipschitz continuous with $\g = \gamma
\|x_j-x_0\|_2^2$.

Suppose $g'(0) > \g/2$. Then $|g'(0)-g'(t)| \le \g t \Longrightarrow
g'(0) - \g t \le g'(t)$, and the line $w=g'(0)-\g t$ intersects the $t$-axis
at $\tilde t=g'(0)/\g > 1/2$. $\tilde t<1$ necessarily, since by Rolle's
Theorem there exists $0<z<1$ such that $g'(z)=0$ and so $g'(0) - \g z \le
g'(z) = 0$. Now
$${g'(0)^2\over  2\g} = {g'(0)\tilde t\over2} = \int_0^{\tilde t}
(g'(0)-\g t)dt \le \int_0^{\tilde t} g'(t)dt = g(\tilde t),$$
and
$${-g'(0)^2\over 2\g} < g'(0) - {g'(0)^2\over 2\g} - \g/2 =
{(1-\tilde t)(g'(0)-\g)\over 2} = \int_{\tilde t}^1 (g'(0)-\g t)dt
\le \int_{\tilde t}^1 g'(t)dt = -g(\tilde t),$$
a contradiction for the value of $g(\tilde t)$. A similar contradiction arises
for $g'(0)<-\g/2$. Therefore $|g'(0)| \le \g/2$.

In terms of $f$,
$$\bigl|\langle \nabla f(x_0)-c,x_j-x_0\rangle\bigr| = |g'(0)| \le \gamma
\|x_j-x_0\|_2^2/2,$$
which holds for all $1\le j\le d$.  Finally, using {\it Lemma 2},
$$\|\nabla f(x_0)-c\|_2^2 \le {d(\gamma k^2/2)^2\over\sigma_d^2}
\Longrightarrow
\|\nabla f(x_0)-c\|_2 \le {\sqrt{d}\,\gamma k^2\over 2\sigma_d}.$$

\bye
